src/cbor/raw/pulse/everparse/CBOR.Pulse.Raw.Serialized.fst
@@ -1,6 +1,7 @@
 module CBOR.Pulse.Raw.Serialized
 open CBOR.Spec.Raw.Base
-open Pulse.Lib.Pervasives
+open CBOR.Pulse.Raw.Iterator
+open CBOR.Pulse.Raw.Iterator.Serialized
 
 open Pulse.Lib.Slice open Pulse.Lib.Pervasives open Pulse.Lib.Trade
 open CBOR.Spec.Raw.Format
@@ -58,3 +59,101 @@ fn cbor_match_serialized_tagged_get_payload
   res
 }
 ```
+  
+let cbor_serialized_array_iterator = cbor_raw_serialized_iterator 
+
+let cbor_serialized_array_iterator_match = cbor_raw_serialized_iterator_match serialize_raw_data_item
+
+module LP = LowParse.Pulse.VCList
+
+```pulse
+ghost
+fn cbor_match_serialized_array_elim
+  (c: cbor_serialized)
+  (pm: perm)
+  (r: raw_data_item { Array? r })
+  requires
+    cbor_match_serialized_array c pm r
+  ensures exists* pm' .
+    pts_to_serialized (LP.serialize_nlist (U64.v (Array?.len r).value) serialize_raw_data_item) c.cbor_serialized_payload #pm' (Array?.v r) **
+    trade
+      (pts_to_serialized (LP.serialize_nlist (U64.v (Array?.len r).value) serialize_raw_data_item) c.cbor_serialized_payload #pm' (Array?.v r))
+      (cbor_match_serialized_array c pm r)
+{
+  unfold (cbor_match_serialized_array c pm r);
+  unfold (cbor_match_serialized_payload_array c.cbor_serialized_payload (pm `perm_mul` c.cbor_serialized_perm) (Array?.v r));
+  with pm' . assert (pts_to_serialized (LP.serialize_nlist (U64.v (Array?.len r).value)  serialize_raw_data_item) c.cbor_serialized_payload #pm' (Array?.v r));
+  ghost fn aux (_: unit)
+    requires emp ** (pts_to_serialized (LP.serialize_nlist (U64.v (Array?.len r).value)  serialize_raw_data_item) c.cbor_serialized_payload #pm' (Array?.v r))
+    ensures (cbor_match_serialized_array c pm r)
+  {
+    fold (cbor_match_serialized_payload_array c.cbor_serialized_payload (pm `perm_mul` c.cbor_serialized_perm) (Array?.v r));
+    fold (cbor_match_serialized_array c pm r);
+  };
+  intro_trade _ _ _ aux
+}
+```
+
+#set-options "--print_implicits"
+
+```pulse
+fn cbor_serialized_array_iterator_init
+  (c: cbor_serialized)
+  (#pm: perm)
+  (#r: Ghost.erased raw_data_item { Array? r })
+requires
+    (cbor_match_serialized_array c pm r)
+returns res: cbor_serialized_array_iterator
+ensures
+    (exists* p .
+      cbor_serialized_array_iterator_match p res (Array?.v r) **
+      trade
+        (cbor_serialized_array_iterator_match p res (Array?.v r))
+        (cbor_match_serialized_array c pm r)
+    )
+{
+  cbor_match_serialized_array_elim c pm r;
+  with p . assert (
+    (pts_to_serialized (LowParse.Spec.VCList.serialize_nlist (U64.v (Array?.len (Ghost.reveal r)).value)
+          serialize_raw_data_item)
+      c.cbor_serialized_payload
+      #p
+      (Array?.v (Ghost.reveal r)))
+  );
+  let res : cbor_serialized_array_iterator = {
+    s = c.cbor_serialized_payload;
+    len = U64.v (Array?.len r).value;
+  };
+  Trade.rewrite_with_trade
+    (pts_to_serialized (LowParse.Spec.VCList.serialize_nlist (U64.v (Array?.len (Ghost.reveal r)).value)
+          serialize_raw_data_item)
+      c.cbor_serialized_payload
+      #p
+      (Array?.v (Ghost.reveal r)))
+    (pts_to_serialized (LowParse.Spec.VCList.serialize_nlist (Ghost.reveal res.len)
+          serialize_raw_data_item)
+      res.s
+      #p
+      (Array?.v (Ghost.reveal r))      
+  )
+  ;
+  Trade.trans _ _ (cbor_match_serialized_array c pm r);
+  cbor_raw_serialized_iterator_fold serialize_raw_data_item p res (Array?.v r);
+  Trade.trans _ _ (cbor_match_serialized_array c pm r);
+  fold (cbor_serialized_array_iterator_match p res (Array?.v r));
+  res
+}
+```
+
+let cbor_serialized_array_iterator_is_empty = cbor_raw_serialized_iterator_is_empty _
+
+inline_for_extraction
+```pulse
+fn cbor_serialized_array_iterator_next_cont (_: unit)
+: cbor_raw_serialized_iterator_next_cont #cbor_raw #raw_data_item #parse_raw_data_item_kind #parse_raw_data_item serialize_raw_data_item cbor_match
+= (x: _) (#pm: _) (#v: _) {
+  cbor_read x
+}
+```
+
+let cbor_serialized_array_iterator_next sq = cbor_raw_serialized_iterator_next _ (jump_raw_data_item sq) cbor_match (cbor_serialized_array_iterator_next_cont ())
